equivalence.dfy
@@ -1,10 +1,10 @@
-include "lemmas.dfy"
+// include "lemmas.dfy"
 include "common.dfy"
 include "steps.dfy"
 
 
 module Equivalence{
-    import opened Lemmas
+    // import opened Lemmas
     import opened Common
     import opened Steps
     ghost predicate AreEquivalent(bf_program: Program, bf_state: State, ir_program: IntermediateRep, input: seq<char>, inputPtr: int)
@@ -45,12 +45,50 @@ module Equivalence{
     ghost predicate EquivalentReps(p: Program, s: State, ir: IntermediateRep)
     requires valid_program(p)
     requires state_reqs(s)
+    requires valid_ir(ir)
+    requires valid_input(ir.input) 
     {
-        // true
-        //Idea: forall i:: 0 <= i < |ir| ==> if program can transition from i to i+1, then ir can as well
-        forall i:: 0 <= i < |ir.commands| ==> exists p': Program, s': State, irS: State, ir': IntermediateRep:: valid_program(p') && state_reqs(s')  && program_k_max_steps(p, s, p', s', i) && state_reqs(irS) //&& ir_k_steps(ir, s, ir', irS, i) //&& s'==irS
+        //Idea: forall values, from any linear location in the program or in the code, they should transition to the same spot
+        // Will call this from any state as well
+(        forall i:: within_ir_range(i, ir) ==> exists p': Program, s': State, ir': IntermediateRep, s1: State:: valid_program(p') && aligned_programs(p, p') && valid_state(s, s') && state_reqs(s')  && program_k_max_steps(p, s, p', s', i) && state_reqs(s1) && valid_state(s, s1) && valid_ir(ir') && valid_input(ir'.input) && ir_step(IntermediateRep(ir.commands, i, ir.input), s, ir', s1) && s'==s1 )
     }
 
+    ghost predicate lockstep(p: Program, s: State, ir: IntermediateRep)
+    requires valid_program(p)
+    requires state_reqs(s)
+    requires valid_ir(ir)
+    requires valid_input(ir.input)
+    {
+        valid_program(p) && valid_ir(ir) && state_reqs(s) &&
+        exists p': Program, s': State, ir': IntermediateRep ::
+        valid_program(p') && state_reqs(s')&& valid_ir(ir')&& valid_input(ir'.input)&& valid_state(s, s')&& aligned_programs(p, p') &&
+        max_steps( p, s, p', s') &&
+        ir_step(ir, s, ir', s')     
+    }
+
+ 
+ghost predicate aligned_instructions(p: Program, ir: IntermediateRep)
+    requires valid_program(p)
+    requires valid_ir(ir)
+    {
+        (|Changes(p)| == |ir.commands|)
+        && forall i:: 0<=i<|ir.commands| ==>(
+            0<=Changes(p)[i] < |p.commands| &&
+               match ir.commands[i]
+                case Inc(k) => (p.commands[Changes(p)[i]] in ['+', '-'] && (k>= 0 ==> ((p.commands[Changes(p)[i]]=='+') && k==count_consecutive_symbols(p, Changes(p)[i]))) && (k<0 ==> (p.commands[Changes(p)[i]]=='-')&&(-k)==count_consecutive_symbols(p, Changes(p)[i]))
+                )
+                case Move(k) => 
+                (p.commands[Changes(p)[i]] in ['>', '<'] && (k>= 0 ==> ((p.commands[Changes(p)[i]]=='>') && k==count_consecutive_symbols(p, Changes(p)[i]))) && (k<0 ==> (p.commands[Changes(p)[i]]=='<')&&(-k)==count_consecutive_symbols(p, Changes(p)[i])))
+                case UserInput => p.commands[Changes(p)[i]] == ','
+                case Print => p.commands[Changes(p)[i]] == '.'
+                case Jump(dest, direction) => ((p.commands[Changes(p)[i]] == ']' && direction == false) || (p.commands[Changes(p)[i]] == '[' && direction == true))
+        
+        )
+        // (p.pointer == |p.commands| && ir.pointer == |ir.commands|) ||
+        // (p.pointer < |p.commands| && ir.pointer < |ir.commands| &&
+        
+        //  )
+    } 
 
 }
 
