steps.dfy
@@ -8,7 +8,7 @@ module Steps{
     requires valid_program(p) && valid_program(p') 
     requires state_reqs(s)
     {
-        0 <= p.pointer < |p.commands| && 0 <= p'.pointer < |p'.commands| && p.commands == p'.commands && 
+        0 <= p.pointer < |p.commands| && 0 <= p'.pointer <= |p'.commands| && p.commands == p'.commands && 
         p.commands != [] ==> //TODO: how to get user input
         match p.commands[p.pointer]
             case '+' => 
@@ -52,7 +52,7 @@ module Steps{
                     && (forall i :: 0 <= i < |s.memory| && i != s.pointer ==> (s.memory[i] == s'.memory[i]))
                     && (|p.input| > 0 ==> (s'.memory[s.pointer] == p.input[0] as int && p'.input == p.input[1..]))
                     && (|p.input| == 0 ==> (p'.input == p.input && s'.memory[s.pointer]==' ' as int))
-                    && pointer_moved_up(p, p')
+                    && pointer_moved_up(p, p')&& s'.output == s.output
                 )
             case default => false
     }
@@ -67,17 +67,17 @@ module Steps{
     {
         if ir.pointer == |ir.commands| then ir' == ir && s' == s
         else 
-        (ir.pointer < |ir.commands| && ir.commands != [] ==> //TODO: how to get user input
+        (ir.pointer < |ir.commands| && ir.commands != [] ==> 
         match ir.commands[ir.pointer]
             case Inc(n) => 
-                0 <= s.pointer < |s.memory| && s.pointer == s'.pointer && |s.memory| == |s'.memory| 
+                0 <= s.pointer < |s.memory| && s.pointer == s'.pointer && |s.memory| == |s'.memory|  && s.output == s'.output
                 && (forall i :: 0 <= i < |s.memory| && i != s.pointer ==> (s.memory[i] == s'.memory[i]))
                 // && ((s.memory[s.pointer]+n >= 255) ==> s'.memory[s.pointer] == s.memory[s.pointer]+n%255)
                 && s'.memory[s.pointer] == (s.memory[s.pointer]+n)%256 && ir_moved_up(ir, ir')
             case Move(n) => 
                 0 <= s.pointer < |s.memory| && s.memory == s'.memory && 0 <= s'.pointer < |s.memory| 
                 && ((s.pointer + n >= |s.memory|) ==> s'.pointer == |s.memory|-1)
-                && ((s.pointer + n <= 0) ==> s'.pointer == 0)
+                && ((s.pointer + n <= 0) ==> s'.pointer == 0) && s.output == s'.output
                 && ((0 <= s.pointer + n < |s.memory|) ==> s'.pointer == s.pointer+n) 
             case Jump(dest, direction) =>
                 (ir_moved_up(ir, ir') && ir.commands == ir'.commands && ir.input == ir'.input && s == s') 
@@ -92,7 +92,7 @@ module Steps{
                     && (forall i :: 0 <= i < |s.memory| && i != s.pointer ==> (s.memory[i] == s'.memory[i]))
                     && (|ir.input| > 0 ==> s'.memory[s.pointer] == ir.input[0] as int && ir'.input==ir.input[1..])
                     && (|ir.input| == 0 ==> s'.memory[s.pointer] == ' ' as int && ir'.input==ir.input)
-                    && ir_moved_up(ir, ir')
+                    && ir_moved_up(ir, ir') && s'.output == s.output
                 )
         )
     }
@@ -105,31 +105,49 @@ module Steps{
     {
         (p.pointer == |p.commands| && p==p' && s==s') || (p.pointer < |p.commands| &&
         match p.commands[p.pointer]
-            case '+' | '-' =>
+            case '+' =>
                 s.pointer == s'.pointer&&
-                |s.memory| == |s'.memory| &&
+                |s.memory| == |s'.memory| && s'.output == s.output&&
                 (p.pointer < p'.pointer)&&
-                (forall i:: (p.pointer<=i< p'.pointer ==>  p.commands[i] in ['+', '-']))
-                && (p'.pointer == |p.commands| || (p'.pointer < |p.commands| ==> !(p.commands[p'.pointer] in ['+', '-'])))
-                && (s'.memory[s.pointer] == (s.memory[s.pointer]+count_commands(p, p', ['+', '-']))%256)
+                (forall i:: (p.pointer<=i< p'.pointer ==>  p.commands[i] == '+'))
+                && (p'.pointer == |p.commands| || (p'.pointer < |p.commands| ==> !(p.commands[p'.pointer] == '+')))
+                && (s'.memory[s.pointer] == (s.memory[s.pointer]+ p'.pointer-p.pointer)%256)
                 && (forall i:: (0 <= i < |s.memory|  && i != s.pointer) ==> s.memory[i] == s'.memory[i])
-            case '>' | '<' =>
+            case '-' =>
+                s.pointer == s'.pointer&&
+                |s.memory| == |s'.memory| && s'.output == s.output&&
                 (p.pointer < p'.pointer)&&
-                (forall i:: (p.pointer<=i< p'.pointer ==>  p.commands[i] in ['>', '<']))
-                && (p'.pointer == |p.commands| || (p'.pointer < |p.commands| ==> !(p.commands[p'.pointer] in ['<', '>'])))
+                (forall i:: (p.pointer<=i< p'.pointer ==>  p.commands[i] == '-'))
+                && (p'.pointer == |p.commands| || (p'.pointer < |p.commands| ==> !(p.commands[p'.pointer] == '-')))
+                && (s'.memory[s.pointer] == (s.memory[s.pointer]+ p.pointer-p'.pointer)%256)
+                && (forall i:: (0 <= i < |s.memory|  && i != s.pointer) ==> s.memory[i] == s'.memory[i])
+            case '>' =>
+                |s.memory| == |s'.memory| && s'.output == s.output&&
+                (p.pointer < p'.pointer)&&
+                (forall i:: (p.pointer<=i< p'.pointer ==>  p.commands[i] == '>'))
+                && (p'.pointer == |p.commands| || (p'.pointer < |p.commands| ==> !(p.commands[p'.pointer] == '>')))
                 && (s'.memory == s.memory)
-                && (0 <= s.pointer+count_commands(p, p', ['>', '<']) < |s.memory| ==> s'.pointer == s.pointer + count_commands(p, p', ['>', '<']))
-                && (0 > s.pointer+count_commands(p, p', ['>', '<']) ==> s'.pointer == 0)
-                && (|s.memory|<= s.pointer+count_commands(p, p', ['>', '<']) ==> s'.pointer == |s.memory|-1)
+                && (0 <= s.pointer+p'.pointer-p.pointer < |s.memory| ==> s'.pointer == s.pointer + p'.pointer-p.pointer)
+                // && (0 > s.pointer+count_commands(p, p', ['>', '<']) ==> s'.pointer == 0)
+                && ((|s.memory|<= s.pointer+p'.pointer-p.pointer) ==> s'.pointer == |s.memory|-1)
+            case '<' =>
+                |s.memory| == |s'.memory| && s'.output == s.output&&
+                (p.pointer < p'.pointer)&&
+                (forall i:: (p.pointer<=i< p'.pointer ==>  p.commands[i] == '<'))
+                && (p'.pointer == |p.commands| || (p'.pointer < |p.commands| ==> !(p.commands[p'.pointer] == '<')))
+                && (s'.memory == s.memory)
+                && (0 <= s.pointer-p'.pointer+p.pointer < |s.memory| ==> s'.pointer == s.pointer - p'.pointer+p.pointer)
+                // && (0 > s.pointer+count_commands(p, p', ['>', '<']) ==> s'.pointer == 0)
+                && ((0 >= s.pointer-p'.pointer+p.pointer) ==> s'.pointer == 0)
             case ',' | '.' =>
                 program_step(s, p, s', p')
             case '[' =>
-            (0 <= s.pointer < |s.memory| && 0 <= s'.pointer < |s.memory| )
+            (s==s' )
                 && pointer_moved_up(p,p')
                 // && (s.memory[s.pointer]== 0 ==> (p'.pointer > p.pointer && p'.commands[p'.pointer-1]== ']' && valid_loop(p.commands[p.pointer+1.. p'.pointer-1])))    //Need to add forall to make sure that at the soonest ]
             case ']' =>
                 (
-                    (0 <= s.pointer < |s.memory| && 0 <= s'.pointer <= |s.memory| )
+                    (s==s')
                     && (pointer_moved_up(p, p'))
                     // && (s.memory[s.pointer] > 0 ==> (0 < p'.pointer < p.pointer && p'.commands[p'.pointer-1]== '[' && valid_loop(p.commands[p'.pointer.. p.pointer-1])))
                 )
@@ -137,31 +155,42 @@ module Steps{
     }
 
 
-function count_commands(p: Program, p': Program, symbols: seq<char>): int
-    requires p.pointer <= p'.pointer <= |p.commands|
-    requires |symbols| == 2
-    requires |p.commands| > 0
-    requires aligned_programs(p, p')
-    decreases p'.pointer-p.pointer
-{
-    if p.pointer == p'.pointer then 0
-    // else if p.pointer + 1 >= p'.pointer then 0
-    else
-        assert p.pointer < |p.commands|;
-        (if p.commands[p.pointer] in symbols then
-            (if p.commands[p.pointer] == '+' then 1 else -1)
-         else 0) +
-         count_commands(p.(pointer := p.pointer + 1), p', symbols)
-}
-
+// function count_commands(p: Program, p': Program, symbol: char): int
+//     requires p.pointer <= p'.pointer <= |p.commands|
+//     requires |p.commands| > 0
+//     requires aligned_programs(p, p')
+//     decreases p'.pointer-p.pointer
+// {
+//     if p.pointer == p'.pointer then 0
+//     // else if p.pointer + 1 >= p'.pointer then 0
+//     else
+//         assert p.pointer < |p.commands|;
+//         (if p.commands[p.pointer] == symbol then
+//             1) +
+//          count_commands(p.(pointer := p.pointer + 1), p', symbols)
+// }
 
     ghost predicate program_k_max_steps(p: Program, s: State, p': Program, s': State, k: int)
+    requires 0<= k
+    requires valid_program(p)
+    requires valid_program(p')
+    requires aligned_programs(p, p')
+    requires state_reqs(s)
+    requires state_reqs(s')
+    requires valid_state(s, s')
+    {
+        (k < |Changes(p)| ==> 0<=Changes(p)[k] < |p.commands| && max_steps(Program(p.commands, Changes(p)[k], p.input), s, p', s'))
+        &&
+        (k >= |Changes(p)| ==> max_steps(Program(p.commands, |p.commands|, p.input), s, p', s'))
+    }
+
+/*    ghost predicate program_k_max_steps(p: Program, s: State, p': Program, s': State, k: int)
     decreases k
     requires 0<= k
     requires valid_program(p)
     requires state_reqs(s)
     {
-    if k==0 then
+    if k==0 then 
         p == p' && s == s' 
     else 
         exists p'': Program, s'': State:: (valid_state(s, s'') && state_reqs(s'') && aligned_programs(p, p'') && valid_program(p'') && max_steps(p, s, p'', s'') &&
@@ -172,8 +201,6 @@ function count_commands(p: Program, p': Program, symbols: seq<char>): int
     decreases k
     requires 0<= k
     // requires valid_program(p)
-    requires 0 <= ir.pointer
-    requires 0<= ir'.pointer
     requires state_reqs(s)
     requires valid_ir(ir)
     requires valid_input(ir.input)
@@ -187,5 +214,20 @@ function count_commands(p: Program, p': Program, symbols: seq<char>): int
         ir_k_steps(ir'', s'', ir', s', k-1))
     }
 
+    ghost predicate StepsForBoth(p: Program, s: State, ir: IntermediateRep)
+    requires valid_program(p)
+    requires state_reqs(s)
+    requires valid_ir(ir)
+    requires valid_input(ir.input)
+    {
+        // true
+        //Idea: forall i:: 0 <= i < |ir| ==> if program can transition from i to i+1, then ir can as well
+        // forall i:: 0 <= i < |ir.commands| ==> exists p': Program, s': State, irS: State, ir': IntermediateRep:: valid_program(p') && state_reqs(s')  && program_k_max_steps(p, s, p', s', i) && state_reqs(irS) && valid_ir(ir') && valid_input(ir'.input) && ir_k_steps(ir, s, ir', irS, i) //&& s'==irS
+// (        forall i:: 0 <= i < |ir.commands| ==> exists p': Program, s': State:: valid_program(p') && state_reqs(s')  && program_k_max_steps(p, s, p', s', i)
+// )        && forall i:: 0 <= i < |ir.commands| ==> exists ir': IntermediateRep, s1: State:: state_reqs(s1) && valid_ir(ir') && valid_input(ir'.input) && ir_k_steps(ir, s, ir', s1, i)
+
+(        forall i:: 0 <= i < |ir.commands| ==> exists p': Program, s': State, ir': IntermediateRep, s1: State:: valid_program(p') && state_reqs(s')  && program_k_max_steps(p, s, p', s', i) && state_reqs(s1) && valid_ir(ir') && valid_input(ir'.input) && ir_k_steps(ir, s, ir', s1, i))
+    }
+*/
 
 }
