lemmas.dfy
@@ -1,10 +1,317 @@
 include "common.dfy"
 include "steps.dfy"
+include "equivalence.dfy"
+
 module Lemmas{
     import opened Common
     import opened Steps
+    import opened Equivalence
 
-lemma MaxKIRSteps(ir: IntermediateRep, s: State, k: int) 
+    lemma and_implies_one(p: Program, s: State, p': Program, s': State)
+    requires ( |s.memory| == |s'.memory| && s'.output == s.output&&
+                (p.pointer < p'.pointer) && 0 <= p.pointer < p'.pointer <= |p.commands| &&
+                (forall i:: (p.pointer<=i< p'.pointer ==>  p.commands[i] == '>'))
+                && (p'.pointer == |p.commands| || (p'.pointer < |p.commands| ==> !(p.commands[p'.pointer] == '>')))
+                && (s'.memory == s.memory)
+                && (0 <= s.pointer+p'.pointer-p.pointer < |s.memory| ==> s'.pointer == s.pointer + p'.pointer-p.pointer)
+                && ((|s.memory|<= s.pointer+p'.pointer-p.pointer) ==> s'.pointer == |s.memory|-1))
+    ensures (forall i:: (p.pointer<=i< p'.pointer ==>  p.commands[i] == '>'))
+    {}
+
+    lemma AlignmentMeansEquivalence(p: Program, s: State, ir: IntermediateRep)
+    requires valid_program(p)
+    requires state_reqs(s)
+    requires valid_ir(ir)
+    requires valid_input(ir.input) 
+    requires ir.input == p.input;
+    requires valid_input(p.input)
+    requires aligned_instructions(p, ir)
+    ensures EquivalentReps(p, s, ir)
+    {
+      var indices := Changes(p);      
+      forall i | within_ir_range(i, ir)
+      ensures exists p': Program, s': State, ir': IntermediateRep, sIR: State:: valid_program(p') && aligned_programs(p, p') && valid_state(s, s') && state_reqs(s')  && program_k_max_steps(p, s, p', s', i) && state_reqs(sIR) && valid_state(s, sIR) && valid_ir(ir') && valid_input(ir'.input) && ir_step(IntermediateRep(ir.commands, i, ir.input), s, ir', sIR) && s'==sIR 
+
+      {
+        var index := indices[i];
+        var currIr := IntermediateRep(ir.commands, i, ir.input);
+        match ir.commands[i] 
+          case Inc(k) =>{
+            assert p.commands[index] in ['+', '-'];
+            var p_by_k := Program(p.commands, index, p.input);
+            MaxSteps(p_by_k, s);
+            assert exists p': Program, s': State ::  valid_program(p') &&  state_reqs(s') &&  valid_state(s, s') &&  aligned_programs(p_by_k, p') && max_steps(p_by_k, s, p', s')  && valid_input(p'.input);
+            var p': Program, s': State :| valid_program(p') &&  state_reqs(s') &&  valid_state(s, s') &&  aligned_programs(p_by_k, p') && max_steps(p_by_k, s, p', s')  && valid_input(p'.input);
+            assert forall j:: p_by_k.pointer <= j < p'.pointer ==> p_by_k.commands[indices[i]] == p_by_k.commands[j];
+            if k >= 0{
+              assert k==count_consecutive_symbols(p, index); 
+              assert p.commands[index] == '+';
+              assert index+k < |p.commands| ==> (p.commands[index] != p.commands[index+k]);
+              assert forall j:: index <= j < index+k ==> p.commands[j] == p.commands[index]; 
+              assert index == p_by_k.pointer;
+              assert p'.pointer - p_by_k.pointer==k;
+              IrStep(currIr, s);
+              var ir': IntermediateRep, sIR :|valid_state(s, sIR) && state_reqs(sIR) && in_sync_irs(currIr, ir') && valid_ir(ir') && ir_step(currIr, s, ir', sIR) && valid_input(ir'.input);
+              assert ir_step(currIr, s, ir', sIR);
+              
+              assert s.pointer == sIR.pointer;
+              assert s.pointer == s'.pointer;
+              assert sIR.memory[sIR.pointer] == (s.memory[sIR.pointer]+k)%256;
+              assert max_steps(p_by_k, s, p', s');
+              assert p_by_k.commands[p_by_k.pointer]=='+';
+              assert s'.memory[s'.pointer] == (s.memory[s.pointer]+ p'.pointer-p_by_k.pointer)%256;
+              assert p'.pointer - p_by_k.pointer==k;
+              assert s'.memory[s'.pointer] == (s.memory[s.pointer]+k)%256;
+              assert s'.memory == sIR.memory;
+              assert s'.output == s.output;
+              assert sIR.output == s.output;
+              assert s'.output == sIR.output;
+              assert s'.pointer == sIR.pointer; 
+              assert valid_program(p') && aligned_programs(p, p') && valid_state(s, s') && state_reqs(s');
+              assert i < |Changes(p)|;
+              assert p_by_k == Program(p.commands, Changes(p)[i], p.input);
+              assert max_steps(p_by_k, s, p', s');
+              assert max_steps(Program(p.commands, Changes(p)[i], p.input), s, p', s');
+              assert program_k_max_steps(p, s, p', s', i);
+              assert state_reqs(sIR) && valid_state(s, sIR) && valid_ir(ir') && valid_input(ir'.input) && ir_step(IntermediateRep(ir.commands, i, ir.input), s, ir', sIR);
+              assert sIR == s';
+              assert valid_program(p') && aligned_programs(p, p') && valid_state(s, s') && state_reqs(s')  && program_k_max_steps(p, s, p', s', i) && state_reqs(sIR) && valid_state(s, sIR) && valid_ir(ir') && valid_input(ir'.input) && ir_step(IntermediateRep(ir.commands, i, ir.input), s, ir', sIR) && s'==sIR ;
+            }else{
+              assert -k==count_consecutive_symbols(p, index); 
+              assert p.commands[index] == '-';
+              assert index-k < |p.commands| ==> (p.commands[index] != p.commands[index-k]);
+              assert forall j:: index <= j < index+k ==> p.commands[j] == p.commands[index]; 
+              assert index == p_by_k.pointer;
+              assert p'.pointer - p_by_k.pointer==-k;
+              IrStep(currIr, s);
+              var ir': IntermediateRep, sIR :|valid_state(s, sIR) && state_reqs(sIR) && in_sync_irs(currIr, ir') && valid_ir(ir') && ir_step(currIr, s, ir', sIR) && valid_input(ir'.input);
+              assert ir_step(currIr, s, ir', sIR);
+              
+              assert s.pointer == sIR.pointer;
+              assert s.pointer == s'.pointer;
+              assert sIR.memory[sIR.pointer] == (s.memory[sIR.pointer]+k)%256;
+              assert max_steps(p_by_k, s, p', s');
+              assert p_by_k.commands[p_by_k.pointer]=='-';
+              assert s'.memory[s'.pointer] == (s.memory[s.pointer]- p'.pointer+p_by_k.pointer)%256;
+              assert p'.pointer - p_by_k.pointer==-k;
+              assert s'.memory[s'.pointer] == (s.memory[s.pointer]+k)%256;
+              assert s'.memory == sIR.memory;
+              assert s'.output == s.output;
+              assert sIR.output == s.output;
+              assert s'.output == sIR.output;
+              assert s'.pointer == sIR.pointer; 
+              assert valid_program(p') && aligned_programs(p, p') && valid_state(s, s') && state_reqs(s');
+              assert i < |Changes(p)|;
+              assert p_by_k == Program(p.commands, Changes(p)[i], p.input);
+              assert max_steps(p_by_k, s, p', s');
+              assert max_steps(Program(p.commands, Changes(p)[i], p.input), s, p', s');
+              assert program_k_max_steps(p, s, p', s', i);
+              assert state_reqs(sIR) && valid_state(s, sIR) && valid_ir(ir') && valid_input(ir'.input) && ir_step(IntermediateRep(ir.commands, i, ir.input), s, ir', sIR);
+              assert sIR == s';
+              assert valid_program(p') && aligned_programs(p, p') && valid_state(s, s') && state_reqs(s')  && program_k_max_steps(p, s, p', s', i) && state_reqs(sIR) && valid_state(s, sIR) && valid_ir(ir') && valid_input(ir'.input) && ir_step(IntermediateRep(ir.commands, i, ir.input), s, ir', sIR) && s'==sIR ;
+                        
+            }
+            // assert forall j:: index <= j < index+k ==> p.commands[j] == p.commands[index];
+            // assert p_by_k.commands==p.commands;
+            // assert count_consecutive_symbols(p, index)==count_consecutive_symbols(p_by_k, index);
+           
+            // assert forall j:: 0<=j<k ==> (index+j < |p.commands|) && p.commands[index+j] == p.commands[index];
+
+          } 
+          case Move(k) =>{
+            assert p.commands[index] in ['>', '<'];
+            var p_by_k := Program(p.commands, index, p.input);
+            MaxSteps(p_by_k, s);
+            assert exists p': Program, s': State ::  valid_program(p') &&  state_reqs(s') &&  valid_state(s, s') &&  aligned_programs(p_by_k, p') && max_steps(p_by_k, s, p', s')  && valid_input(p'.input);
+            var p': Program, s': State :| valid_program(p') &&  state_reqs(s') &&  valid_state(s, s') &&  aligned_programs(p_by_k, p') && max_steps(p_by_k, s, p', s')  && valid_input(p'.input);
+            assert max_steps(p_by_k,s, p', s');
+            if k >= 0{
+              assert max_steps(p_by_k,s, p', s');
+
+              assert (|s.memory| == |s'.memory| && s'.output == s.output&&
+                (p_by_k.pointer < p'.pointer)&&
+                (forall i:: (p_by_k.pointer<=i< p'.pointer ==>  p_by_k.commands[i] == '>'))
+                && (p'.pointer == |p_by_k.commands| || (p'.pointer < |p_by_k.commands| ==> !(p_by_k.commands[p'.pointer] == '>')))
+                && (s'.memory == s.memory)
+                && (0 <= s.pointer+p'.pointer-p_by_k.pointer < |s.memory| ==> s'.pointer == s.pointer + p'.pointer-p_by_k.pointer))
+                // && (0 > s.pointer+count_commands(p, p', ['>', '<']) ==> s'.pointer == 0)
+                && ((|s.memory|<= s.pointer+p'.pointer-p_by_k.pointer) ==> s'.pointer == |s.memory|-1);
+              // assert max_steps(p_by_k, s, p', s') ==> (forall i:: (p_by_k.pointer<=i< p'.pointer ==>  p_by_k.commands[i] == '>'));
+              assert (forall i:: (p_by_k.pointer<=i< p'.pointer ==>  p_by_k.commands[i] == '>'));
+              // assert forall j:: p_by_k.pointer <= j < p'.pointer ==> p_by_k.commands[j] == '>';
+              assert index+k < |p.commands| ==> (p.commands[index] != p.commands[index+k]);
+              assert forall j:: index <= j < index+k ==> p.commands[j] == p.commands[index]; 
+              assert index == p_by_k.pointer;
+              assert p'.pointer - p_by_k.pointer==k;
+              IrStep(currIr, s);
+              var ir': IntermediateRep, sIR :|valid_state(s, sIR) && state_reqs(sIR) && in_sync_irs(currIr, ir') && valid_ir(ir') && ir_step(currIr, s, ir', sIR) && valid_input(ir'.input);
+              assert ir_step(currIr, s, ir', sIR);
+              if (s.pointer + k >= |s.memory|){
+                assert sIR.pointer == |s.memory|-1;
+                assert s'.pointer == |s.memory|-1;
+
+              } else if (s.pointer +k < 0){
+                assert sIR.pointer == 0;
+                assert s'.pointer == 0;
+              } else {
+                assert sIR.pointer == s.pointer +k;
+                assert s'.pointer == s.pointer +k;
+              }
+              assert sIR.memory == s.memory;
+              assert max_steps(p_by_k, s, p', s');
+              assert p_by_k.commands[p_by_k.pointer]=='>';
+              assert s'.memory==s'.memory;
+              assert p'.pointer - p_by_k.pointer==k;
+              // assert s'.memory[s'.pointer] == (s.memory[s.pointer]+k)%256;
+              assert s'.memory == sIR.memory;
+              assert s'.output == s.output;
+              assert sIR.output == s.output;
+              assert s'.output == sIR.output;
+              assert s'.pointer == sIR.pointer; 
+              assert valid_program(p') && aligned_programs(p, p') && valid_state(s, s') && state_reqs(s');
+              assert i < |Changes(p)|;
+              assert p_by_k == Program(p.commands, Changes(p)[i], p.input);
+              assert max_steps(p_by_k, s, p', s');
+              assert max_steps(Program(p.commands, Changes(p)[i], p.input), s, p', s');
+              assert program_k_max_steps(p, s, p', s', i);
+              assert state_reqs(sIR) && valid_state(s, sIR) && valid_ir(ir') && valid_input(ir'.input) && ir_step(IntermediateRep(ir.commands, i, ir.input), s, ir', sIR);
+              assert sIR == s';
+              assert valid_program(p') && aligned_programs(p, p') && valid_state(s, s') && state_reqs(s')  && program_k_max_steps(p, s, p', s', i) && state_reqs(sIR) && valid_state(s, sIR) && valid_ir(ir') && valid_input(ir'.input) && ir_step(IntermediateRep(ir.commands, i, ir.input), s, ir', sIR) && s'==sIR ;
+            }else{
+              assert max_steps(p_by_k,s, p', s');
+
+              assert (|s.memory| == |s'.memory| && s'.output == s.output&&
+                (p_by_k.pointer < p'.pointer)&&
+                (forall i:: (p_by_k.pointer<=i< p'.pointer ==>  p_by_k.commands[i] == '<'))
+                && (p'.pointer == |p_by_k.commands| || (p'.pointer < |p_by_k.commands| ==> !(p_by_k.commands[p'.pointer] == '<')))
+                && (s'.memory == s.memory)
+                && (0 <= s.pointer-p'.pointer+p_by_k.pointer < |s.memory| ==> s'.pointer == s.pointer - p'.pointer+p_by_k.pointer))
+                // && (0 > s.pointer+count_commands(p, p', ['>', '<']) ==> s'.pointer == 0)
+                && ((0>= s.pointer-p'.pointer+p_by_k.pointer) ==> s'.pointer == 0);
+              // assert max_steps(p_by_k, s, p', s') ==> (forall i:: (p_by_k.pointer<=i< p'.pointer ==>  p_by_k.commands[i] == '>'));
+              assert (forall i:: (p_by_k.pointer<=i< p'.pointer ==>  p_by_k.commands[i] == '<'));
+              // assert forall j:: p_by_k.pointer <= j < p'.pointer ==> p_by_k.commands[j] == '>';
+              assert index-k < |p.commands| ==> (p.commands[index] != p.commands[index-k]);
+              assert forall j:: index <= j < index-k ==> p.commands[j] == p.commands[index]; 
+              assert index == p_by_k.pointer;
+              assert -p'.pointer + p_by_k.pointer==k;
+              IrStep(currIr, s);
+              var ir': IntermediateRep, sIR :|valid_state(s, sIR) && state_reqs(sIR) && in_sync_irs(currIr, ir') && valid_ir(ir') && ir_step(currIr, s, ir', sIR) && valid_input(ir'.input);
+              assert ir_step(currIr, s, ir', sIR);
+              if (s.pointer + k >= |s.memory|){
+                assert sIR.pointer == |s.memory|-1;
+                assert s'.pointer == |s.memory|-1;
+
+              } else if (s.pointer +k < 0){
+                assert sIR.pointer == 0;
+                assert s'.pointer == 0;
+              } else {
+                assert sIR.pointer == s.pointer +k;
+                assert s'.pointer == s.pointer +k;
+              }
+              assert sIR.memory == s.memory;
+              assert max_steps(p_by_k, s, p', s');
+              assert p_by_k.commands[p_by_k.pointer]=='<';
+              assert s'.memory==s'.memory;
+              assert p'.pointer - p_by_k.pointer==-k;
+              // assert s'.memory[s'.pointer] == (s.memory[s.pointer]+k)%256;
+              assert s'.memory == sIR.memory;
+              assert s'.output == s.output;
+              assert sIR.output == s.output;
+              assert s'.output == sIR.output;
+              assert s'.pointer == sIR.pointer; 
+              assert valid_program(p') && aligned_programs(p, p') && valid_state(s, s') && state_reqs(s');
+              assert i < |Changes(p)|;
+              assert p_by_k == Program(p.commands, Changes(p)[i], p.input);
+              assert max_steps(p_by_k, s, p', s');
+              assert max_steps(Program(p.commands, Changes(p)[i], p.input), s, p', s');
+              assert program_k_max_steps(p, s, p', s', i);
+              assert state_reqs(sIR) && valid_state(s, sIR) && valid_ir(ir') && valid_input(ir'.input) && ir_step(IntermediateRep(ir.commands, i, ir.input), s, ir', sIR);
+              assert sIR == s';
+              assert valid_program(p') && aligned_programs(p, p') && valid_state(s, s') && state_reqs(s')  && program_k_max_steps(p, s, p', s', i) && state_reqs(sIR) && valid_state(s, sIR) && valid_ir(ir') && valid_input(ir'.input) && ir_step(IntermediateRep(ir.commands, i, ir.input), s, ir', sIR) && s'==sIR ;
+                      
+            }
+          
+          }
+          case Print =>{
+            var p_by_k := Program(p.commands, index, p.input);
+            MaxSteps(p_by_k, s);
+            assert exists p': Program, s': State ::  valid_program(p') &&  state_reqs(s') &&  valid_state(s, s') &&  aligned_programs(p_by_k, p') && max_steps(p_by_k, s, p', s')  && valid_input(p'.input);
+            var p': Program, s': State :| valid_program(p') &&  state_reqs(s') &&  valid_state(s, s') &&  aligned_programs(p_by_k, p') && max_steps(p_by_k, s, p', s')  && valid_input(p'.input);
+            assert max_steps(p_by_k,s, p', s');
+            IrStep(currIr, s);  
+            var ir': IntermediateRep, sIR :|valid_state(s, sIR) && state_reqs(sIR) && in_sync_irs(currIr, ir') && valid_ir(ir') && ir_step(currIr, s, ir', sIR) && valid_input(ir'.input);
+            assert sIR.memory == s.memory;
+            assert sIR == s';          
+          }
+          case UserInput =>{
+            var p_by_k := Program(p.commands, index, p.input);
+            MaxSteps(p_by_k, s);
+            assert exists p': Program, s': State ::  valid_program(p') &&  state_reqs(s') &&  valid_state(s, s') &&  aligned_programs(p_by_k, p') && max_steps(p_by_k, s, p', s')  && valid_input(p'.input);
+            var p': Program, s': State :| valid_program(p') &&  state_reqs(s') &&  valid_state(s, s') &&  aligned_programs(p_by_k, p') && max_steps(p_by_k, s, p', s')  && valid_input(p'.input);
+            assert max_steps(p_by_k,s, p', s');
+            IrStep(currIr, s);  
+            var ir': IntermediateRep, sIR :|valid_state(s, sIR) && state_reqs(sIR) && in_sync_irs(currIr, ir') && valid_ir(ir') && ir_step(currIr, s, ir', sIR) && valid_input(ir'.input);
+            // assert sIR.memory == s.memory;
+            assert sIR == s';          
+          }
+          
+          case _ => {assume false;}
+          assert exists p': Program, s': State, ir': IntermediateRep, sIR: State:: valid_program(p') && aligned_programs(p, p') && valid_state(s, s') && state_reqs(s')  && program_k_max_steps(p, s, p', s', i) && state_reqs(sIR) && valid_state(s, sIR) && valid_ir(ir') && valid_input(ir'.input) && ir_step(IntermediateRep(ir.commands, i, ir.input), s, ir', sIR) && s'==sIR ;
+
+      }
+
+      assert EquivalentReps(p, s, ir);
+
+    }
+
+
+/*lemma CombineForAlls(p: Program, s: State, ir: IntermediateRep)
+requires valid_program(p)
+  requires valid_ir(ir)
+  requires valid_input(p.input)
+  requires state_reqs(s)
+  requires valid_input(ir.input)
+  requires 0 <= s.pointer < |s.memory|
+  requires exists ir': IntermediateRep, s': State ::
+    valid_state(s, s') && state_reqs(s') && in_sync_irs(ir, ir') && valid_ir(ir') &&
+    ir_step(ir, s, ir', s') && valid_input(ir'.input)
+  requires exists p_next: Program, s_next: State ::
+    valid_state(s, s_next) && state_reqs(s_next) && aligned_programs(p, p_next) && 
+    valid_program(p_next) && max_steps(p, s, p_next, s_next) && valid_input(p_next.input)  ensures forall k :: 0 <= k ==> exists p': Program, s': State, s2: State, ir': IntermediateRep ::
+    valid_program(p') && state_reqs(s') && program_k_max_steps(p, s, p', s', k) &&
+    state_reqs(s2) && valid_ir(ir') && valid_input(ir'.input) && ir_k_steps(ir, s, ir', s2, k)
+{
+  var k := 0;
+  while (true) // Conceptual loop over all non-negative k
+    invariant 0 <= k;
+    invariant forall i :: 0 <= i <= k ==> (exists si: State, s3i: State, pi: Program, iri: IntermediateRep ::
+      valid_program(pi) && state_reqs(si) && program_k_max_steps(p, s, pi, si, i) &&
+      state_reqs(s3i) && valid_ir(iri) && valid_input(iri.input) && ir_k_steps(ir, s, iri, s3i, i));
+  {
+    MaxKIRSteps(ir, s, k);
+    MaxKSteps(p, s, k);
+
+    var p_k: Program, s_k: State :| valid_program(p_k) && state_reqs(s_k) &&
+                                    program_k_max_steps(p, s, p_k, s_k, k);
+    var ir_k: IntermediateRep, s2_k: State :| valid_ir(ir_k) && state_reqs(s2_k) && valid_input(ir_k.input) &&
+                                        ir_k_steps(ir, s, ir_k, s2_k, k);
+
+    // Need to show that the invariant is maintained for k + 1
+    assert exists sk_plus_1: State, s3k_plus_1: State, pk_plus_1: Program, irk_plus_1: IntermediateRep ::
+      valid_program(pk_plus_1) && state_reqs(sk_plus_1) && program_k_max_steps(p, s, pk_plus_1, sk_plus_1, k + 1) &&
+      state_reqs(s3k_plus_1) && valid_ir(irk_plus_1) && valid_input(irk_plus_1.input) && ir_k_steps(ir, s, irk_plus_1, s3k_plus_1, k + 1);
+
+    k := k + 1;
+  }
+  // The postcondition should follow from the loop invariant.
+  assert forall k_final :: 0 <= k_final ==> exists p': Program, s': State, s2': State, ir': IntermediateRep ::
+    valid_program(p') && state_reqs(s') && program_k_max_steps(p, s, p', s', k_final) &&
+    state_reqs(s2') && valid_ir(ir') && valid_input(ir'.input) && ir_k_steps(ir, s, ir', s2', k_final);
+}*/
+
+
+/*lemma MaxKIRSteps(ir: IntermediateRep, s: State, k: int) 
 //   requires 0 <= p.pointer <= |p.commands|
   requires valid_ir(ir)
   requires state_reqs(s)
@@ -44,7 +351,7 @@ decreases k
 
     
     }
-  }
+  }*/
 
 
 lemma IrStep(ir: IntermediateRep, s: State)
@@ -122,7 +429,7 @@ lemma IrStep(ir: IntermediateRep, s: State)
             
     }
 }
-lemma MaxKSteps(p: Program, s: State, k: int) 
+/*lemma MaxKSteps(p: Program, s: State, k: int) 
   requires 0 <= p.pointer <= |p.commands|
   requires valid_program(p)
   requires state_reqs(s)
@@ -161,7 +468,7 @@ decreases k
 
     
     }
-  }
+  }*/
 
 
 lemma MaxSteps(p: Program, s: State)
@@ -223,16 +530,10 @@ lemma MaxStepsPlusMinus(p: Program, s: State)
   ensures exists p': Program, s': State :: valid_program(p') && state_reqs(s') && valid_state(s, s') && aligned_programs(p, p') && max_steps(p, s, p', s')  && valid_input(p'.input)
 {
     var i := p.pointer+1;
-    var count := 0;
-    if p.commands[p.pointer] == '+'{
-        count := 1;
-    } else{
-        count := -1;
-    }
-    while i < |p.commands| && p.commands[i] in ['+', '-']
+    while i < |p.commands| && p.commands[i] ==p.commands[p.pointer]
     decreases |p.commands|-i
     invariant i <= |p.commands|
-    invariant forall j:: p.pointer <= j < i ==> p.commands[j] in ['+', '-']
+    invariant forall j:: p.pointer <= j < i ==> p.commands[j] == p.commands[p.pointer]
     {
         i := i+1;
     }
@@ -250,18 +551,26 @@ lemma MaxStepsPlusMinus(p: Program, s: State)
     assert |s2|==0;*/
     var p' := Program(p.commands, i, p.input);
     // assert enough_input(p');
-    count := count_commands(p, p', ['+', '-']);
-    mem :=   mem[..s.pointer] + [(s.memory[s.pointer]+count)%256] + mem[s.pointer+1..];
+    // count := count_commands(p, p', ['+', '-']);
+    if p.commands[p.pointer] == '+'{
+      mem :=   mem[..s.pointer] + [(s.memory[s.pointer]+p'.pointer-p.pointer)%256] + mem[s.pointer+1..];
+      assert mem[s.pointer] == (s.memory[s.pointer]+p'.pointer-p.pointer)%256;
+    }else if p.commands[p.pointer]=='-'{
+      mem :=   mem[..s.pointer] + [(s.memory[s.pointer]-p'.pointer+p.pointer)%256] + mem[s.pointer+1..];
+      assert mem[s.pointer] == (s.memory[s.pointer]-p'.pointer+p.pointer)%256;
+
+
+    }
     var s' := StateValue(s.pointer, mem, s.output);
     assert valid_program(p') && aligned_programs(p, p');
     assert state_reqs(s');
-    assert (forall i:: (p.pointer<=i< p'.pointer ==>  p.commands[i] in ['+', '-']));
-    assert (p'.pointer == |p.commands| || (p'.pointer < |p.commands| ==> !(p.commands[p'.pointer] in ['+', '-'])));
+    assert (forall i:: (p.pointer<=i< p'.pointer ==>  p.commands[i] ==p.commands[p.pointer]));
+    assert (p'.pointer == |p.commands| || (p'.pointer < |p.commands| ==> !(p.commands[p'.pointer] == p.commands[p.pointer])));
     assert (forall i:: (0 <= i < |s.memory|  && i != s.pointer) ==> s.memory[i] == s'.memory[i]);
-    assert count == count_commands(p, p', ['+', '-']);
+    // assert count == count_commands(p, p', ['+', '-']);
     assert valid_input(p'.input);
-    assert s'.memory[s.pointer] == (s.memory[s.pointer]+count)%256;
-    assert (s'.memory[s.pointer] == (s.memory[s.pointer]+count_commands(p, p', ['+', '-']))%256);
+    assert p.commands[p.pointer] == '+' ==> s'.memory[s.pointer] == (s.memory[s.pointer]+p'.pointer-p.pointer)%256;
+    assert p.commands[p.pointer] == '-'==>(s'.memory[s.pointer] == (s.memory[s.pointer]-p'.pointer+p.pointer)%256);
     assert max_steps(p, s, p', s');
 }
 
@@ -407,23 +716,39 @@ lemma MaxStepsMove(p: Program, s: State)
   requires valid_input(p.input)
   ensures exists p': Program, s': State :: valid_program(p') && state_reqs(s') && valid_state(s, s') && aligned_programs(p, p') && max_steps(p, s, p', s') && valid_input(p'.input)
 {
-    var i := p.pointer+1;
-    var count := 0;
-    if p.commands[p.pointer] == '+'{
-        count := 1;
-    } else{
-        count := -1;
-    }
-    while i < |p.commands| && p.commands[i] in ['>', '<']
+  var i := p.pointer+1;
+    while i < |p.commands| && p.commands[i] ==p.commands[p.pointer]
     decreases |p.commands|-i
     invariant i <= |p.commands|
-    invariant forall j:: p.pointer <= j < i ==> p.commands[j] in ['>', '<']
+    invariant forall j:: p.pointer <= j < i ==> p.commands[j] == p.commands[p.pointer]
     {
         i := i+1;
     }
+    var mem := s.memory;
+    // var newVal := s.memory[s.pointer];
+    // assert enough_input(p);
+    /*assert forall j:: p.pointer <= j < i ==> p.commands[j] != ',';
+    var s2 := set j| p.pointer <= j < i && p.commands[j]==',';
+    assert forall j:: p.pointer <= j < i ==> (!(j in s2));
+    var s3 := set j | i <= j < |p.commands| && p.commands[j] == ',';
+    var s4 := set j | p.pointer <= j < |p.commands| && p.commands[j]==',';
+    assert s4 == s2+s3;
+    assert |s4| == |s2|+|s3|;
+    // assert forall j :: p.pointer <= j < i ==> !(j in s2);
+    assert |s2|==0;*/
     var p' := Program(p.commands, i, p.input);
+    // assert enough_input(p');
+    // count := count_commands(p, p', ['+', '-']);
+    var count := 0;
+    if p.commands[p.pointer] == '>'{
+      count := p'.pointer-p.pointer;
+      // mem :=   mem[..s.pointer] + [(s.memory[s.pointer]+p'.pointer-p.pointer)%256] + mem[s.pointer+1..];
+    }else if p.commands[p.pointer]=='<'{
+      count := p.pointer-p'.pointer;
+      // mem :=   mem[..s.pointer] + [(s.memory[s.pointer]-p'.pointer+p.pointer)%256] + mem[s.pointer+1..];
+
+    }
     
-    count := count_commands(p, p', ['>', '<']);
     var point := s.pointer;
     assert 0 <= point;
     if point + count >= |s.memory|{
@@ -437,10 +762,9 @@ lemma MaxStepsMove(p: Program, s: State)
     var s' := StateValue(point, s.memory, s.output);
     assert valid_program(p') && aligned_programs(p, p');
     assert state_reqs(s');
-    assert (forall i:: (p.pointer<=i< p'.pointer ==>  p.commands[i] in ['>', '<']));
-    assert (p'.pointer == |p.commands| || (p'.pointer < |p.commands| ==> !(p.commands[p'.pointer] in ['>', '<'])));
+    assert (forall i:: (p.pointer<=i< p'.pointer ==>  p.commands[i] == p.commands[p.pointer]));
+    assert (p'.pointer == |p.commands| || (p'.pointer < |p.commands| ==> !(p.commands[p'.pointer] == p.commands[p.pointer])));
     assert (forall i:: (0 <= i < |s.memory|  && i != s.pointer) ==> s.memory[i] == s'.memory[i]);
-    assert count == count_commands(p, p', ['>', '<']);
     assert max_steps(p, s, p', s');
 }
 
@@ -499,11 +823,107 @@ lemma AllLessThanLast(s: seq<int>)
 {
 }
 
-lemma ExistsValidState(s: State)
-requires state_reqs(s)
-ensures exists s': State:: state_reqs(s')
-{
-    // exists s': State:: s' == s
-}
+// lemma Lockstep(p: Program, s: State, ir: IntermediateRep)
+//     requires valid_program(p)
+//     requires state_reqs(s)
+//     requires valid_ir(ir)
+//     requires valid_input(ir.input)
+//     requires ir.input == p.input
+//     // requires valid_input(p.input)
+//     requires aligned_instructions(p, ir)
+//     // ensures lockstep(p, s, ir)
+//     {
+//       if ir.pointer == |ir.commands|{
+//         assert lockstep(p, s, ir);
+//       }else{
+//         match ir.commands[ir.pointer] 
+//           case UserInput =>{
+            
+//             assert aligned_instructions(p, ir) ==> p.commands[p.pointer] == ',';
+//             IrStep(ir, s);
+//             MaxSteps(p, s);
+//             var s': State, ir': IntermediateRep :| state_reqs(s') && valid_ir(ir') && valid_state(s, s') && ir_step(ir, s, ir', s');
+//             var s2: State, p': Program :| state_reqs(s2) && valid_program(p') && aligned_programs(p, p') && valid_state(s, s2) && max_steps(p, s, p', s2);
+//             assert p.commands[p.pointer] == ',';
+//             assert max_steps(p, s, p', s2);
+//             assert program_step(s, p, s2, p');
+//             assert p.commands != [];
+//             assert match p.commands[p.pointer] 
+//               case ',' => true
+//               case _ => false;
+//             assert 0 <= p.pointer < |p.commands| && 0 <= p'.pointer <= |p'.commands| && p.commands == p'.commands && (
+//                                  0 <= s.pointer < |s.memory| && s.pointer == s2.pointer && |s.memory| == |s2.memory| 
+//                                 && (forall i :: 0 <= i < |s.memory| && i != s.pointer ==> (s.memory[i] == s2.memory[i]))
+//                                 && (|p.input| > 0 ==> (s2.memory[s.pointer] == p.input[0] as int && p'.input == p.input[1..]))
+//                                 && (|p.input| == 0 ==> (p'.input == p.input && s2.memory[s.pointer]==' ' as int))
+//                                 && pointer_moved_up(p, p')
+//                              );
+//             assert (forall i :: 0 <= i < |s.memory| && i != s.pointer ==> (s.memory[i] == s2.memory[i])&& (|p.input| > 0 ==> (s2.memory[s.pointer] == p.input[0] as int))
+//                                 && (|p.input| == 0 ==> (s2.memory[s.pointer]==' ' as int)));
+
+//             assert valid_ir(ir');
+//             assert ir_step(ir, s, ir', s');
+//             assert                     0 <= s.pointer < |s.memory| && s.pointer == s'.pointer && |s.memory| == |s'.memory| 
+//                     && (forall i :: 0 <= i < |s.memory| && i != s.pointer ==> (s.memory[i] == s'.memory[i]))
+//                     && (|ir.input| > 0 ==> s'.memory[s.pointer] == ir.input[0] as int && ir'.input==ir.input[1..])
+//                     && (|ir.input| == 0 ==> s'.memory[s.pointer] == ' ' as int && ir'.input==ir.input)
+//                     && ir_moved_up(ir, ir') && s2.output == s.output;
+//             assert (forall i :: 0 <= i < |s.memory| && i != s.pointer ==> (s.memory[i] == s'.memory[i]))
+//                     && (|ir.input| > 0 ==> s'.memory[s.pointer] == ir.input[0] as int)
+//                     && (|ir.input| == 0 ==> s'.memory[s.pointer] == ' ' as int)&& s'.output == s.output;
+//             assert s'.memory == s2.memory;
+//             assert s'.pointer == s2.pointer;
+//             assert s'.output == s2.output;
+//             assert p.commands[p.pointer] == ',';
+//             assert s' == s2;
+
+//             assert lockstep(p, s, ir);
+//           }
+//           case Print =>{
+//             assert aligned_instructions(p, ir) ==> p.commands[p.pointer] == '.';
+//             IrStep(ir, s);
+//             MaxSteps(p, s);
+//             var s': State, ir': IntermediateRep :| state_reqs(s') && valid_ir(ir') && valid_state(s, s') && ir_step(ir, s, ir', s');
+//             var s2: State, p': Program :| state_reqs(s2) && valid_program(p') && aligned_programs(p, p') && valid_state(s, s2) && max_steps(p, s, p', s2);
+//             assert p.commands[p.pointer] == '.';
+//             assert max_steps(p, s, p', s2);
+//             assert program_step(s, p, s2, p');
+//             assert p.commands != [];
+//             assert match p.commands[p.pointer] 
+//               case '.' => true
+//               case _ => false;
+//             assert s.memory == s2.memory && s.pointer == s2.pointer 
+//                 // && (0 <= s.pointer < |s.memory| && 0 <= s'.pointer < |s.memory| )
+//                 && s2.output == s.output + [s.memory[s.pointer] as char];
+//             assert valid_ir(ir');
+//             assert ir_step(ir, s, ir', s');
+//             assert s.memory == s'.memory && s.pointer == s'.pointer && s'.output == s.output + [s.memory[s.pointer]as char];
+//             assert s'==s2;
+//             assert lockstep(p, s, ir);
+//           }
+//           case Move(k) =>{
+//             MaxSteps(p, s);
+//             var s2: State, p': Program :| state_reqs(s2) && valid_program(p') && aligned_programs(p, p') && valid_state(s, s2) && max_steps(p, s, p', s2);
+
+//             // assert k == count_commands(p, p', ['+', '-']);
+//           }
+//           // case Inc(k) =>{}
+//           case Jump(dest, direction)=>{
+//             IrStep(ir, s);
+//             MaxSteps(p, s);
+//             var s': State, ir': IntermediateRep :| state_reqs(s') && valid_ir(ir') && valid_state(s, s') && ir_step(ir, s, ir', s');
+//             assert valid_ir(ir');
+//             assert ir_step(ir, s, ir', s');
+//             assert s'==s;
+//             var s2: State, p': Program :| state_reqs(s2) && valid_program(p') && aligned_programs(p, p') && valid_state(s, s2) && max_steps(p, s, p', s2);
+//             assert s2==s;
+//             assert s2==s'; 
+//             assert lockstep(p, s, ir);
+//           }
+//           case _ => {assume false;}
+//       }
+      
+
+//     }
 
 }
