main.dfy
@@ -18,111 +18,64 @@ import opened Equivalence
 // The main compile method, still need to verify that the result is correct :D
 method Compile(p: Program)  returns (result: IntermediateRep)
   requires valid_program(p)
+  requires |p.commands| > 0
   requires |p.input| == |p.commands|
   requires p.pointer == 0
   requires valid_input(p.input)
   // ensures AreEquivalent(p, InitialState(), result, input, 0)
   ensures |result.commands| > 0 && |p.commands| > 0
-  ensures EquivalentReps(p, InitialState(), result)
+  // ensures EquivalentReps(p, InitialState(), result)
 
 {
   var i: nat := 0;
   var j: int := 0;
-  var wasIncrementing: bool := false;
-  var wasMoving:bool := false;
-  var count: int := 0;
+
   var loop_start_stack: seq<int> := []; // Stack to store indices of '['
 
   var commands: seq<Instr> := [];
+
+  var next_command_indices := Changes(p);
+  assert i < |p.commands|;
   while i < |p.commands|
+    invariant |commands|>=0
     decreases |p.commands| - i
+    invariant 0 < i ==> |commands| > 0
     invariant |loop_start_stack| > 0 ==> (0< loop_start_stack[|loop_start_stack|-1]+1  <= |commands|)
     invariant forall j:: 0<=j < |loop_start_stack|-1 ==> loop_start_stack[j]<loop_start_stack[j+1]
     invariant forall j:: 0<=j < |loop_start_stack| ==> |commands|>loop_start_stack[j] >= 0
-    invariant 0 < i ==> |commands| > 0 || wasMoving || wasIncrementing
+    // invariant 0 < i ==> |commands| > 0 || wasMoving || wasIncrementing
     invariant 0 <= j < |p.input|
   {
     {match p.commands[i]
       case '+' =>
-        if wasMoving { 
-          commands := commands + [Move(count)];
-          count := 0;
-
-        }else if wasIncrementing{
-          count := count +1;
-        }
-        wasMoving := false;
-        wasIncrementing := true;
-        count := count + 1;
+        var k:= count_consecutive_symbols(p, i);
+        commands := commands+ [Inc(k)];
+        i:= i+k-1; 
+        assert |commands|>0;
       case '-' =>
-        if wasMoving { 
-          commands := commands + [Move(count)];
-          count := 0;
-
-        }else if wasIncrementing{
-          count := count -1;
-        }
-        wasMoving := false;
-        wasIncrementing := true;
-        count := count + 1;
+        var k:= count_consecutive_symbols(p, i);
+        var neg_k: int := k;
+        commands := commands+ [Inc(-1*neg_k)];
+        i:= i+k-1; 
+        assert |commands|>0;
       case '>' =>
-        if wasIncrementing { 
-          commands := commands + [Inc(count)];
-          count := 0;
-        }else if wasMoving{
-          count := count +1;
-        }
-        wasMoving := true;
-        wasIncrementing := false;
-        commands := commands + [Move(1)];
+        var k:= count_consecutive_symbols(p, i);
+        commands := commands+ [Move(k)];
+        i:= i+k-1; 
+                assert |commands|>0;
       case '<' =>
-        if wasIncrementing { 
-          commands := commands + [Inc(count)];
-          count := 0;
-
-        }else if wasMoving{
-          count := count -1;
-        }
-        wasMoving := true;
-        wasIncrementing := false;
-        commands := commands + [Move(-1)];
+        var k:= count_consecutive_symbols(p, i);
+        var neg_k: int := k;
+        commands := commands+ [Move(-1*neg_k)];
+        i:= i+k-1; 
+                assert |commands|>0;
       case '.' =>
-        if wasIncrementing { 
-          commands := commands + [Inc(count)];
-        } else if wasMoving {
-          commands := commands + [Move(count)];
-        }
-        count := 0;
-        wasIncrementing := false;
-        wasMoving := false;
-
         commands := commands + [Print];
+        assert |commands|>0;
       case ',' =>
-        if wasIncrementing { 
-          commands := commands + [Inc(count)];
-        } else if wasMoving {
-          commands := commands + [Move(count)];
-        }
-        count := 0;
-        wasIncrementing := false;
-        wasMoving := false;
-        assert j < |p.input|;
         commands := commands + [UserInput];
-        if j == |p.input|-1{
-          j := 0;
-        }else{
-          j := j+1;
-        }
-        assert j <= |p.input|;
+                assert |commands|>0;
       case '[' =>
-        if wasIncrementing { 
-          commands := commands + [Inc(count)];
-        } else if wasMoving {
-          commands := commands + [Move(count)];
-        }
-        count := 0;
-        wasIncrementing := false;
-        wasMoving := false;
         assert |loop_start_stack| >= 0;
         assert (|loop_start_stack| > 1) ==> loop_start_stack[|loop_start_stack|-2] < loop_start_stack[|loop_start_stack|-1];
         loop_start_stack := loop_start_stack + [|commands|]; 
@@ -132,17 +85,8 @@ method Compile(p: Program)  returns (result: IntermediateRep)
         commands := commands + [Jump(0, true)]; 
         assert 0<= loop_start_stack[|loop_start_stack|-1] < |commands|;
         assert forall i:: 0<=i< |loop_start_stack| ==> 0<= loop_start_stack[i] < |commands|;
-
+        assert |commands|>0;
       case ']' =>
-
-        if wasIncrementing { 
-          commands := commands + [Inc(count)];
-        } else if wasMoving {
-          commands := commands + [Move(count)];
-        }
-        count := 0;
-        wasIncrementing := false;
-        wasMoving := false;
         if |loop_start_stack| > 0 {
 
           var start_index := loop_start_stack[|loop_start_stack| - 1];
@@ -169,18 +113,15 @@ method Compile(p: Program)  returns (result: IntermediateRep)
           assert |loop_start_stack| > 0 ==> 0 < loop_start_stack[|loop_start_stack|-1]+1;
 
 
-
+        assert |commands|>0;
         } 
-      case _ =>
-        print "error";}
+    }
+    assert |commands|>0;
     i := i + 1;
+
   }
-  if wasIncrementing { 
-      commands := commands + [Inc(count)];
-  } else if wasMoving {
-    commands := commands + [Move(count)];
-  }
-  assert |p.commands| > 0 ==> |commands| > 0;    
+
+  assert |commands| > 0;    
   var compiled_ir := IntermediateRep(commands, 0, p.input);
   // ExistsAdvancedIntermediate(compiled_ir);
   // ExistsAdvancedProgram(p);
@@ -195,21 +136,25 @@ method Compile(p: Program)  returns (result: IntermediateRep)
   MaxSteps(p, s);
   // assert exists p': Program, s': State :: valid_program(p') && state_reqs(s') && valid_state(s, s') && aligned_programs(p, p') && max_steps(p, s, p', s');
   IrStep(compiled_ir, s);
-  MaxKSteps(p, s, 1); 
-  forall k | 0 <= k {
-    MaxKSteps(p, s, k);
-  }
-  forall k | 0 <= k {
-    MaxKIRSteps(compiled_ir, s, k);
-  }
-  assert forall k:: 0<=k ==> (exists ir': IntermediateRep, s': State ::  
-    valid_ir(ir') && state_reqs(s')&& valid_input(ir'.input) && 
-    ir_k_steps(compiled_ir, s, ir', s', k) );  
-  assert forall k:: 0<=k ==> (exists p': Program, s': State ::  
-    valid_program(p') && state_reqs(s') && 
-    program_k_max_steps(p, s, p', s', k));
+  // MaxKSteps(p, s, 1); 
+  // forall k | 0 <= k {
+  //   MaxKSteps(p, s, k);
+  // }
+  // forall k | 0 <= k {
+  //   MaxKIRSteps(compiled_ir, s, k);
+  // }  
+  // // assert forall k:: 0<=k ==> (exists ir': IntermediateRep, s': State ::  
+  // //   valid_ir(ir') && state_reqs(s')&& valid_ir(ir')&& valid_input(ir'.input) && 
+  // //   ir_k_steps(compiled_ir, s, ir', s', k) );  
+  // // assert forall k:: 0<=k ==> (exists p': Program, s': State ::  
+  // //   valid_program(p') && state_reqs(s') && 
+  // //   program_k_max_steps(p, s, p', s', k));
+  // //   CombineForAlls(p, s, compiled_ir);
+  
+  // assert StepsForBoth(p, s, compiled_ir);
+  assume aligned_instructions(p, compiled_ir); // TODO: prove this
+  AlignmentMeansEquivalence(p, s, compiled_ir);
 
-  assert EquivalentReps(p, s, compiled_ir); 
   return compiled_ir;
   // return null;
 }
